feat: port plainly lemmas

src/Iris/BI/Plainly.lean
@@ -32,33 +32,34 @@ macro_rules
 delab_rule Plainly.plainlyIf
   | `($_ $p $P) => do ``(iprop(■? $p $(← Iris.BI.unpackIprop P)))
 
-namespace Iris.BI
-open Iris.Std BI
 
 -- FIXME: These names are inconsistent
-class BiPlainly (PROP : Type _) [BI PROP] extends Plainly PROP where
-  [ne : OFE.NonExpansive (Plainly.plainly (PROP := PROP))]
+class BiPlainly (PROP : Type _) [Iris.BI PROP] extends Plainly PROP where
+  [ne : Iris.OFE.NonExpansive (Plainly.plainly (PROP := PROP))]
   mono {P Q : PROP} : iprop(P ⊢ Q) → iprop(■ P ⊢ ■ Q)
   elim_persistently {P : PROP} : iprop(■ P ⊢ <pers> P)
   idemp {P : PROP} : iprop(■ P ⊢ ■ ■ P)
-  plainly_forall {A : Type _} (Ψ : A → PROP) : iprop(∀ a, ■ (Ψ a)) ⊢ ■ (∀ a, Ψ a)
+  -- TODO: How to properly generalize `Type` to `Type _` here? Breaks usages for some reason
+  plainly_forall_2 {A : Type} {Ψ : A → PROP} : iprop(∀ a, ■ (Ψ a)) ⊢ ■ (∀ a, Ψ a)
   plainly_impl_plainly {P Q : PROP} : iprop((■ P → ■ Q) ⊢ ■ (■ P → Q))
   emp_intro {P : PROP} : iprop(P ⊢ ■ emp)
   plainly_absorb {P Q : PROP} : iprop(■ P ∗ Q ⊢ ■ P)
   later_plainly_1 (P : PROP) : iprop(▷ ■ P ⊢ ■ ▷ P)
   later_plainly_2 (P : PROP) : iprop(■ ▷ P ⊢ ▷ ■ P)
 
-class BiPersistentlyImplPlainly (PROP : Type _) [BI PROP] [BiPlainly PROP] where
+class BiPersistentlyImplPlainly (PROP : Type _) [Iris.BI PROP] [BiPlainly PROP] where
   pers_impl_plainly (P Q : PROP) : iprop((■ P → <pers> Q) ⊢ <pers> (■ P → Q))
 
-class BiPlainlyExist (PROP : Type _) [BI PROP] [BiPlainly PROP] where
-  plainly_exist_1 A (Ψ : A → PROP) : iprop(■ (∃ a, Ψ a) ⊢ ∃ a, ■ (Ψ a))
+class BiPlainlyExist (PROP : Type _) [Iris.BI PROP] [BiPlainly PROP] where
+  -- TODO: How to properly generalize `Type` to `Type _` here? Breaks usages for some reason
+  plainly_exist_1 {A : Type} {Ψ : A → PROP} : iprop(■ (∃ a, Ψ a) ⊢ ∃ a, ■ (Ψ a))
+export BiPlainlyExist (plainly_exist_1)
 
--- Internal Eq's
+namespace Iris.BI
+open Iris.Std BI
 
 class Plain {PROP: Type _}  [BI PROP] [Plainly PROP] [BiPlainly PROP] (P : PROP) where
   plain : P ⊢ ■ P
-
 
 section PlainlyLaws
 open BiPlainly
@@ -73,66 +74,39 @@ theorem persistently_elim_plainly : <pers> ■ P ⊣⊢ ■ P :=
   ⟨absorbingly_of_persistently.trans <| sep_symm.trans plainly_absorb,
    idemp.trans elim_persistently⟩
 
-theorem plainly_persistently_elim : ■ <pers> P ⊣⊢ ■ P :=
-  ⟨by
-    apply Entails.trans true_and.2
-    apply Entails.trans
-    · apply and_mono
-      · apply emp_intro
-      · apply BIBase.Entails.rfl
-    apply flip Entails.trans
-    · apply mono
-      apply persistently_and_emp_elim
-    apply Entails.trans and_forall_bool.1
-    apply flip Entails.trans
-    · apply mono
-      apply and_forall_bool.2
-    -- apply Entails.trans
-    -- · apply forall_mono
-    --   intro a
-    --   exact BIBase.Entails.rfl
-    apply flip Entails.trans
-    · rename_i I1 I2
-      -- Universe issue? I guess we neeed sForall
-      have H := @plainly_forall PROP I1 I2
-      sorry
-    all_goals sorry,
-   idemp.trans <| mono elim_persistently⟩
+theorem plainly_persistently_elim : ■ <pers> P ⊣⊢ ■ P := by
+  constructor
+  · refine (true_and.2.trans <| and_mono emp_intro .rfl).trans ?_
+    refine .trans ?_ (mono <| and_forall_bool.2.trans persistently_and_emp_elim)
+    refine and_forall_bool.1.trans ?_
+    refine .trans ?_ plainly_forall_2
+    refine forall_mono ?_
+    exact (Bool.rec .rfl .rfl ·)
+  · exact idemp.trans <| mono elim_persistently
 
-theorem absorbingly_elim_plainly : <absorb> ■ P ⊣⊢ ■ P :=
-  ⟨by
-    apply Entails.trans (absorbingly_mono <| persistently_elim_plainly.2)
-    apply (flip Entails.trans persistently_elim_plainly.1)
-    apply Entails.trans absorbingly_persistently.1
-    apply BIBase.Entails.rfl,
-   by
-    apply flip Entails.trans (absorbingly_mono <| persistently_elim_plainly.1)
-    apply (Entails.trans persistently_elim_plainly.2)
-    apply flip Entails.trans absorbingly_persistently.2
-    apply BIBase.Entails.rfl⟩
+theorem absorbingly_elim_plainly : <absorb> ■ P ⊣⊢ ■ P := by
+  constructor
+  · refine (absorbingly_mono <| persistently_elim_plainly.2).trans ?_
+    refine .trans ?_ persistently_elim_plainly.1
+    exact absorbingly_persistently.1.trans .rfl
+  · refine .trans ?_ (absorbingly_mono persistently_elim_plainly.1)
+    refine persistently_elim_plainly.2.trans ?_
+    exact .trans .rfl absorbingly_persistently.2
 
-theorem plainly_and_sep_elim : ■ P ∧ Q ⊢ (emp ∧ P) ∗ Q := by
-  apply Entails.trans
-  · apply and_mono
-    · apply elim_persistently
-    · apply BIBase.Entails.rfl
-  apply persistently_and_sep_elim_emp
+theorem plainly_and_sep_elim : ■ P ∧ Q ⊢ (emp ∧ P) ∗ Q :=
+  (and_mono elim_persistently .rfl).trans persistently_and_sep_elim_emp
 
-theorem plainly_and_sep_assoc : ■ P ∧ (Q ∗ R) ⊣⊢ (■ P ∧ Q) ∗ R :=
-  ⟨ by
-    apply Entails.trans (and_mono persistently_elim_plainly.2 BIBase.Entails.rfl)
-    apply (flip Entails.trans)
-    · apply sep_mono (and_mono persistently_elim_plainly.1 BIBase.Entails.rfl) BIBase.Entails.rfl
-    apply persistently_and_sep_assoc.1,
-    by
-      apply flip Entails.trans (and_mono persistently_elim_plainly.1 BIBase.Entails.rfl)
-      apply Entails.trans
-      · apply sep_mono (and_mono persistently_elim_plainly.2 BIBase.Entails.rfl) BIBase.Entails.rfl
-      apply persistently_and_sep_assoc.2 ⟩
+theorem plainly_and_sep_assoc : ■ P ∧ (Q ∗ R) ⊣⊢ (■ P ∧ Q) ∗ R := by
+  constructor
+  · refine (and_mono persistently_elim_plainly.2 BIBase.Entails.rfl).trans ?_
+    refine .trans ?_ (sep_mono (and_mono persistently_elim_plainly.1 .rfl) .rfl)
+    exact persistently_and_sep_assoc.1
+  · refine .trans ?_ (and_mono persistently_elim_plainly.1 .rfl)
+    refine (sep_mono (and_mono persistently_elim_plainly.2 .rfl) .rfl).trans ?_
+    exact persistently_and_sep_assoc.2
 
-theorem plainly_and_emp_elim : emp ∧ ■ P ⊢ P := by
-  apply Entails.trans (and_mono BIBase.Entails.rfl elim_persistently)
-  apply persistently_and_emp_elim
+theorem plainly_and_emp_elim : emp ∧ ■ P ⊢ P :=
+  (and_mono .rfl elim_persistently).trans persistently_and_emp_elim
 
 theorem plainly_into_absorbingly : ■ P ⊢ <absorb> P :=
   elim_persistently.trans absorbingly_of_persistently
@@ -146,63 +120,165 @@ theorem plainly_idemp : ■ ■ P ⊣⊢ ■ P :=
 theorem plainly_intro' (H : ■ P ⊢ Q) : ■ P ⊢ ■ Q :=
   plainly_idemp.2.trans <| mono <| H
 
--- theorem plainly_pure φ : ■ ⌜φ⌝ ⊣⊢@{PROP} ⌜φ⌝.
--- theorem plainly_forall {A} (Ψ : A → PROP) : ■ (∀ a, Ψ a) ⊣⊢ ∀ a, ■ (Ψ a).
--- theorem plainly_exist_2 {A} (Ψ : A → PROP) : (∃ a, ■ (Ψ a)) ⊢ ■ (∃ a, Ψ a).
--- theorem plainly_exist `{!BiPlainlyExist PROP} {A} (Ψ : A → PROP) : ■ (∃ a, Ψ a) ⊣⊢ ∃ a, ■ (Ψ a).
+theorem plainly_pure {φ} : ■ ⌜φ⌝ ⊣⊢ (⌜φ⌝ : PROP) := by
+  refine ⟨elim_persistently.trans persistently_elim, ?_⟩
+  refine pure_elim' (fun φ => ?_)
+  apply Entails.trans (Q := «forall» (fun x : Empty => iprop(■ True)))
+  · exact forall_intro Empty.rec
+  · exact plainly_forall_2.trans (mono <| pure_intro φ)
 
-theorem plainly_and : ■ (P ∧ Q) ⊣⊢ ■ P ∧ ■ Q :=
-  ⟨ by sorry, sorry ⟩
-theorem plainly_or_2 : ■ P ∨ ■ Q ⊢ ■ (P ∨ Q) := sorry
--- theorem plainly_or `{!BiPlainlyExist PROP} P Q : ■ (P ∨ Q) ⊣⊢ ■ P ∨ ■ Q.
-theorem plainly_impl : ■ (P → Q) ⊢ ■ P → ■ Q := sorry
--- theorem plainly_emp_2 : emp ⊢@{PROP} ■ emp.
-theorem plainly_sep_dup : ■ P ⊣⊢ ■ P ∗ ■ P :=
-  ⟨ by
-      apply Entails.trans and_self.2
-      apply Entails.trans <| and_mono BIBase.Entails.rfl emp_sep.2
-      apply Entails.trans <| plainly_and_sep_assoc.1
-      apply Entails.trans <| sep_mono and_elim_l BIBase.Entails.rfl
-      apply BIBase.Entails.rfl,
-    by exact plainly_absorb ⟩
+-- TODO: Generalize Type to Type _
+theorem plainly_forall {A : Type} {Ψ : A → PROP} : ■ (∀ a, Ψ a) ⊣⊢ ∀ a, ■ (Ψ a) := 
+  ⟨forall_intro (mono <| forall_elim ·), plainly_forall_2⟩
+
+theorem plainly_exist_2 {A : Sort _} {Ψ : A → PROP} : (∃ a, ■ (Ψ a)) ⊢ ■ (∃ a, Ψ a) :=
+  exists_elim (mono <| exists_intro ·)
+
+-- TODO: Generalize Type to Type _
+theorem plainly_exist [I : BiPlainlyExist PROP] {A : Type} {Ψ : A → PROP} : ■ (∃ a, Ψ a) ⊣⊢ ∃ a, ■ (Ψ a) :=
+  ⟨plainly_exist_1, plainly_exist_2⟩
+
+theorem plainly_and : ■ (P ∧ Q) ⊣⊢ ■ P ∧ ■ Q := by
+  constructor
+  · refine (mono and_forall_bool.mp).trans (.trans ?_ and_forall_bool.mpr)
+    exact plainly_forall.mp.trans (forall_mono (Bool.rec .rfl .rfl ·))
+  · refine (and_forall_bool.mp).trans (.trans ?_ (mono <| and_forall_bool.mpr))
+    refine .trans (forall_mono ?_) plainly_forall.mpr
+    exact (Bool.rec .rfl .rfl ·)
+
+theorem plainly_or_2 : ■ P ∨ ■ Q ⊢ ■ (P ∨ Q) := by
+  refine or_exists_bool.mp.trans (.trans ?_ (mono <| or_exists_bool.mpr))
+  refine .trans (exists_mono ?_) plainly_exist_2
+  exact (Bool.rec .rfl .rfl ·)
+
+theorem plainly_or [BiPlainlyExist PROP] : ■ (P ∨ Q) ⊣⊢ ■ P ∨ ■ Q := by
+  refine ⟨?_, plainly_or_2⟩
+  refine (mono or_exists_bool.mp).trans (.trans ?_ or_exists_bool.mpr)
+  exact plainly_exist_1.trans <| exists_mono (Bool.rec .rfl .rfl ·)
+
+theorem plainly_impl : ■ (P → Q) ⊢ ■ P → ■ Q := by
+  refine imp_intro' <| plainly_and.mpr.trans ?_
+  exact mono imp_elim_r
+
+theorem plainly_emp_2 : (emp : PROP) ⊢ ■ emp := emp_intro
+
+theorem plainly_sep_dup : ■ P ⊣⊢ ■ P ∗ ■ P := by
+  refine ⟨?_, plainly_absorb⟩
+  refine and_self.2.trans ?_
+  refine ((and_mono .rfl emp_sep.2).trans plainly_and_sep_assoc.1).trans ?_
+  exact (sep_mono and_elim_l .rfl).trans .rfl
 
 theorem plainly_and_sep_l_1 : ■ P ∧ Q ⊢ ■ P ∗ Q := by
-  apply Entails.trans <| and_mono BIBase.Entails.rfl emp_sep.2
-  apply Entails.trans <| plainly_and_sep_assoc.1
-  apply Entails.trans <| sep_mono and_elim_l BIBase.Entails.rfl
-  apply BIBase.Entails.rfl
+  refine ((and_mono BIBase.Entails.rfl emp_sep.2).trans plainly_and_sep_assoc.1).trans ?_
+  exact (sep_mono and_elim_l .rfl).trans .rfl
 
 theorem plainly_and_sep_r_1 : P ∧ ■ Q ⊢ P ∗ ■ Q :=
   and_comm.1.trans <| plainly_and_sep_l_1.trans sep_symm
 
--- theorem plainly_True_emp : ■ True ⊣⊢@{PROP} ■ emp.
+theorem plainly_True_emp : ■ True ⊣⊢ ■ (emp : PROP) :=
+  ⟨emp_intro, mono true_intro⟩
 
-theorem plainly_and_sep : ■ (P ∧ Q) ⊢ ■ (P ∗ Q) := sorry
-theorem plainly_affinely_elim : ■ <affine> P ⊣⊢ ■ P := sorry
-theorem intuitionistically_plainly_elim : □ ■ P ⊢ □ P := sorry
-theorem intuitionistically_plainly : □ ■ P ⊢ ■ □ P := sorry
-theorem and_sep_plainly : ■ P ∧ ■ Q ⊣⊢ ■ P ∗ ■ Q := sorry
-theorem plainly_sep_2 : ■ P ∗ ■ Q ⊢ ■ (P ∗ Q) := sorry
--- theorem plainly_sep `{!BiPositive PROP} P Q : ■ (P ∗ Q) ⊣⊢ ■ P ∗ ■ Q.
-theorem plainly_wand : ■ (P -∗ Q) ⊢ ■ P -∗ ■ Q := sorry
-theorem plainly_entails_l : (P ⊢ ■ Q) → P ⊢ ■ Q ∗ P := sorry
-theorem plainly_entails_r : (P ⊢ ■ Q) → P ⊢ P ∗ ■ Q := sorry
-theorem plainly_impl_wand_2 : ■ (P -∗ Q) ⊢ ■ (P → Q) := sorry
-theorem impl_wand_plainly_2 : (■ P -∗ Q) ⊢ (■ P → Q) := sorry
-theorem impl_wand_affinely_plainly : (■ P → Q) ⊣⊢ (<affine> ■ P -∗ Q) := sorry
--- theorem persistently_wand_affinely_plainly `{!BiPersistentlyImplPlainly PROP} P Q : (<affine> ■ P -∗ <pers> Q) ⊢ <pers> (<affine> ■ P -∗ Q).
-theorem plainly_wand_affinely_plainly : (<affine> ■ P -∗ ■ Q) ⊢ ■ (<affine> ■ P -∗ Q) := sorry
+theorem plainly_and_sep : ■ (P ∧ Q) ⊢ ■ (P ∗ Q) := by
+  refine (plainly_and.mp.trans <| (and_mono idemp .rfl).trans plainly_and.mpr).trans ?_
+  refine (mono <| and_mono .rfl emp_sep.mpr).trans ?_
+  refine (mono <| plainly_and_sep_assoc.1).trans ?_
+  refine (mono <| sep_mono and_comm.mp .rfl).trans ?_
+  exact (mono <| sep_mono plainly_and_emp_elim .rfl).trans .rfl
 
+theorem plainly_affinely_elim : ■ <affine> P ⊣⊢ ■ P := by
+  constructor
+  · refine plainly_and.mp.trans ?_
+    refine (and_mono plainly_True_emp.mpr .rfl).trans ?_
+    exact (and_mono plainly_pure.mp .rfl).trans and_elim_r
+  · refine .trans ?_ plainly_and.mpr
+    refine .trans ?_ (and_mono plainly_True_emp.mp .rfl)
+    refine .trans ?_ (and_mono plainly_pure.mpr .rfl)
+    exact and_intro true_intro .rfl
+
+theorem intuitionistically_plainly_elim : □ ■ P ⊢ □ P :=
+  intuitionistically_affinely.mpr.trans <| intuitionistically_mono affinely_plainly_elim
+
+theorem intuitionistically_plainly : □ ■ P ⊢ ■ □ P := by
+  refine (affinely_elim.trans ?_).trans plainly_affinely_elim.mpr
+  exact persistently_elim_plainly.mp.trans plainly_persistently_elim.mpr
+
+theorem and_sep_plainly : ■ P ∧ ■ Q ⊣⊢ ■ P ∗ ■ Q :=
+  ⟨plainly_and_sep_l_1, and_intro plainly_absorb (sep_symm.trans plainly_absorb)⟩
+
+theorem plainly_sep_2 : ■ P ∗ ■ Q ⊢ ■ (P ∗ Q) :=
+  and_sep_plainly.mpr.trans <| plainly_and.mpr.trans plainly_and_sep
+
+theorem plainly_sep [BIPositive PROP] : ■ (P ∗ Q) ⊣⊢ ■ P ∗ ■ Q := by
+  refine ⟨?_, plainly_sep_2⟩
+  refine plainly_affinely_elim.mpr.trans ?_
+  refine (mono <| affinely_sep.mp).trans ?_
+  refine .trans ?_ and_sep_plainly.mp
+  apply (and_intro (mono ?_) (mono ?_))
+  · exact ((sep_mono .rfl affinely_elim_emp).trans sep_emp.mp).trans affinely_elim
+  · exact ((sep_mono affinely_elim_emp .rfl).trans emp_sep.mp).trans affinely_elim
+
+theorem plainly_wand : ■ (P -∗ Q) ⊢ ■ P -∗ ■ Q :=
+  wand_intro <| plainly_sep_2.trans (mono wand_elim_l)
+
+theorem plainly_entails_l (H : P ⊢ ■ Q) : P ⊢ ■ Q ∗ P :=
+  (and_intro H .rfl).trans plainly_and_sep_l_1
+
+theorem plainly_entails_r (H : P ⊢ ■ Q) : P ⊢ P ∗ ■ Q :=
+  (and_intro .rfl H).trans plainly_and_sep_r_1
+
+theorem plainly_impl_wand_2 : ■ (P -∗ Q) ⊢ ■ (P → Q) := by
+  refine plainly_intro' (imp_intro ?_)
+  refine (and_mono .rfl emp_sep.mpr).trans ?_
+  refine plainly_and_sep_assoc.mp.trans ?_
+  refine (sep_mono (and_comm.mp.trans plainly_and_emp_elim) .rfl).trans ?_
+  exact wand_elim_l
+
+theorem impl_wand_plainly_2 : (■ P -∗ Q) ⊢ (■ P → Q) :=
+  imp_intro' <| plainly_and_sep_l_1.trans wand_elim_r
+
+theorem impl_wand_affinely_plainly : (■ P → Q) ⊣⊢ (<affine> ■ P -∗ Q) := by
+  constructor
+  · refine (imp_mono_l persistently_elim_plainly.mp).trans ?_
+    refine intuitionistically_wand.mpr.trans ?_
+    exact wand_mono_l <| affinely_mono persistently_elim_plainly.mpr
+  · refine .trans ?_ (imp_mono_l persistently_elim_plainly.mpr)
+    refine .trans ?_ intuitionistically_wand.mp
+    exact wand_mono_l affinely_of_intuitionistically
+
+theorem persistently_wand_affinely_plainly [BiPersistentlyImplPlainly PROP] :
+    (<affine> ■ P -∗ <pers> Q) ⊢ <pers> (<affine> ■ P -∗ Q) := by
+  refine .trans impl_wand_affinely_plainly.mpr ?_
+  refine .trans ?_ (persistently_mono <| impl_wand_affinely_plainly.mp)
+  exact BiPersistentlyImplPlainly.pers_impl_plainly _ _
+
+theorem plainly_wand_affinely_plainly : (<affine> ■ P -∗ ■ Q) ⊢ ■ (<affine> ■ P -∗ Q) := by
+  refine .trans impl_wand_affinely_plainly.mpr ?_
+  refine .trans ?_ (mono <| impl_wand_affinely_plainly.mp)
+  exact plainly_impl_plainly
 
 section AffineBI
 
 variable [BIAffine PROP]
 
---  theorem plainly_emp : ■ emp ⊣⊢@{PROP} emp.
-theorem plainly_and_sep_l : ■ P ∧ Q ⊣⊢ ■ P ∗ Q := sorry
-theorem plainly_and_sep_r : P ∧ ■ Q ⊣⊢ P ∗ ■ Q := sorry
-theorem plainly_impl_wand : ■ (P → Q) ⊣⊢ ■ (P -∗ Q) := sorry
-theorem impl_wand_plainly : (■ P → Q) ⊣⊢ (■ P -∗ Q) := sorry
+theorem plainly_emp : ■ emp ⊣⊢ (emp : PROP) :=
+  ⟨plainly_elim, plainly_emp_2⟩
+
+theorem plainly_and_sep_l : ■ P ∧ Q ⊣⊢ ■ P ∗ Q :=
+  ⟨plainly_and_sep_l_1, sep_and⟩
+
+theorem plainly_and_sep_r : P ∧ ■ Q ⊣⊢ P ∗ ■ Q := by
+  constructor
+  · exact (and_comm.mp).trans <| plainly_and_sep_l.mp.trans sep_symm
+  · exact sep_symm.trans <| plainly_and_sep_l.mpr.trans and_comm.mpr
+
+theorem plainly_impl_wand : ■ (P → Q) ⊣⊢ ■ (P -∗ Q) := by
+  refine ⟨?_, plainly_impl_wand_2⟩
+  refine plainly_intro' <| wand_intro' ?_
+  refine plainly_and_sep_r.mpr.trans ?_
+  exact (and_mono .rfl plainly_elim).trans imp_elim_r
+
+theorem impl_wand_plainly : (■ P → Q) ⊣⊢ (■ P -∗ Q) :=
+  ⟨imp_wand_1, impl_wand_plainly_2⟩
 
 end AffineBI
 
